semantics/proofs/fpOptPropsScript.sml
@@ -1,0 +1,472 @@
+(**
+  This file contains proofs about the matching and instantiation functions
+  defined in patternScript.sml
+  It also contains some compatibility lemmas for rwAllValTree, the value tree
+  rewriting function
+**)
+
+open fpOptTheory fpValTreeTheory terminationTheory;
+open preamble;
+
+val _ = new_theory "fpOptProps";
+
+Theorem substLookup_substUpdate:
+  ! s n.
+    substLookup s n = NONE ==>
+    ! v. substUpdate n v s = NONE
+Proof
+  Induct_on `s` \\ rpt strip_tac \\ fs[substLookup_def, substUpdate_def]
+  \\ Cases_on `h`
+  \\ fs[substLookup_def]
+  \\ Cases_on `q = n` \\ fs[] \\ res_tac
+  \\ Q.ISPEC_THEN `r` (fn thm => fs[thm]) (CONJUNCT2 substUpdate_def)
+QED
+
+(* Substitutions are only added to but not overwritten *)
+Theorem matchValTree_preserving:
+  ! p s1 s2 v.
+    matchValTree p v s1 = SOME s2 ==>
+    ! n val.
+      substLookup s1 n = SOME val ==> substLookup s2 n = SOME val
+Proof
+  Induct_on `p`
+  \\ rpt strip_tac \\ Cases_on `v`
+  \\ fs[matchValTree_def] \\ rveq
+  \\ fs[option_case_eq] \\ rveq \\ fs[]
+  \\ res_tac \\ fs[substAdd_def]
+  \\ drule substLookup_substUpdate \\ disch_then assume_tac
+  \\ fs[substLookup_def]
+  \\ rename [`substLookup s1 m = SOME _`]
+  \\ Cases_on `n = m` \\ fs[]
+QED
+
+val substMonotone_def = Define `
+  substMonotone s1 s2 =
+    ! n val. substLookup s1 n = SOME val ==> substLookup s2 n = SOME val`;
+
+(* We can add dummy substitutions *)
+Theorem instValTree_weakening:
+  ! p v s1 s2.
+    substMonotone s1 s2 /\
+    instValTree p s1 = SOME v ==>
+    instValTree p s2 = SOME v
+Proof
+  Induct_on `p` \\ rpt strip_tac
+  \\ fs[instValTree_def, substMonotone_def, pair_case_eq, option_case_eq]
+  \\ rveq \\ res_tac \\ fs[]
+QED
+
+(* Sanity lemmas *)
+val valSolve_tac =
+  irule instValTree_weakening
+  \\ asm_exists_tac \\ fs[substMonotone_def]
+  \\ rpt strip_tac
+  \\ imp_res_tac matchValTree_preserving \\ fs[];
+
+Theorem subst_pat_is_val:
+  ! p v s1 s2.
+    matchValTree p v s1 = SOME s2 ==>
+    instValTree p s2 = SOME v
+Proof
+  Induct_on `p`
+  \\ rpt strip_tac \\ fs[]
+  \\ Cases_on `v`
+  \\ fs[matchValTree_def, instValTree_def, option_case_eq]
+  \\ rveq \\ fs[]
+  \\ imp_res_tac substLookup_substUpdate
+  \\ fs[substAdd_def, substLookup_def]
+  \\ res_tac \\ fs[]
+  \\ rpt conj_tac \\ valSolve_tac
+QED
+
+Theorem app_match_sym:
+  ! p s v.
+    instValTree p s = SOME v ==>
+    matchValTree p v s = SOME s
+Proof
+  Induct_on `p`
+  \\ rpt strip_tac
+  \\ fs[ instValTree_def, matchValTree_def, option_case_eq]
+  \\ rveq \\ res_tac
+  \\ fs[matchValTree_def]
+QED
+
+Theorem rwAllValTree_empty_rewrites[simp]:
+  ! canOpt insts v1 v2.
+    rwAllValTree insts canOpt [] v1 = SOME v2 ==>
+    v1 = v2 /\ insts = []
+Proof
+  Induct_on `insts` \\ fs[rwAllValTree_def]
+  \\ ntac 4 strip_tac \\ CCONTR_TAC \\ fs[]
+  \\ Cases_on `h` \\ Cases_on `v1` \\ fs[rwAllValTree_def, nth_def]
+QED
+
+Theorem rwAllValTree_id[simp]:
+  ! canOpt rws v. ? insts. rwAllValTree insts canOpt rws v = SOME v
+Proof
+  rpt strip_tac \\ qexists_tac `[]` \\ EVAL_TAC
+QED
+
+Theorem nth_EL:
+  ! n l x.
+    (nth l n = SOME x) ==> (EL (n-1) l = x /\ (n-1) < LENGTH l)
+Proof
+  Induct_on `l` \\ fs[nth_def] \\ rpt strip_tac
+  >- (Cases_on `n = 1` \\ fs[] \\ rveq
+      \\ res_tac \\ Cases_on `n` \\ fs[]
+      \\ rename [`EL (n - 1) _ = x`]
+      \\ Cases_on `n` \\ fs[])
+  \\ Cases_on `n` \\ fs[]
+  \\ rename [`SUC n < _`] \\ Cases_on `n` \\ fs[]
+  \\ res_tac
+  \\ fs [GSYM ADD1]
+QED
+
+Theorem EL_nth:
+  ! n l x.
+  EL n l = x /\ n < LENGTH l ==> nth l (n+1) = SOME x
+Proof
+  Induct_on `l` \\ fs[nth_def]
+  \\ rpt strip_tac
+  \\ Cases_on `n = 0` \\ fs[]
+  \\ Cases_on `n` \\ fs[] \\ res_tac
+  \\ fs[ADD1]
+QED
+
+Theorem rwAllValTree_up:
+  ! insts canOpt rws1 rws2 v1 v2.
+    set rws1 SUBSET set rws2 /\
+    rwAllValTree insts canOpt rws1 v1 = SOME v2 ==>
+    ?insts2. rwAllValTree insts2 canOpt rws2 v1 = SOME v2
+Proof
+  Induct_on `insts` \\ fs[rwAllValTree_def] \\ rpt strip_tac
+  \\ Cases_on `h` \\ rename1 `RewriteApp pth ind`
+  \\ fs[rwAllValTree_def, option_case_eq]
+  \\ res_tac
+  \\ fs[SUBSET_DEF, MEM_EL] \\ imp_res_tac nth_EL
+  \\ `?n. n < LENGTH rws2 /\ rw = EL n rws2`
+      by (first_x_assum (qspecl_then [`rw`] irule)
+          \\ asm_exists_tac \\ imp_res_tac nth_EL \\ asm_exists_tac \\ fs[])
+  \\ rename [`rwAllValTree insts3 canOpt rws2 v_new = SOME v2`]
+  \\ qexists_tac `RewriteApp pth (n + 1) :: insts3`
+  \\ fs[rwAllValTree_def]
+  \\ `nth rws2 (n+1) = SOME rw` suffices_by (fs[])
+  \\ irule EL_nth \\ fs[]
+QED
+
+Theorem rwAllValTree_comp_unop:
+  ! v vres insts canOpt rws u.
+    rwAllValTree insts canOpt rws v = SOME vres ==>
+    ? insts_new.
+      rwAllValTree insts_new canOpt rws (Fp_uop u v) = SOME (Fp_uop u vres)
+Proof
+  Induct_on `insts` \\ rpt strip_tac
+  \\ fs[rwAllValTree_def]
+  \\ Cases_on `h` \\ fs[rwAllValTree_def, option_case_eq]
+  \\ res_tac
+  \\ first_x_assum (qspec_then `u` assume_tac) \\ fs[]
+  \\ qexists_tac `(RewriteApp (Center f) n):: insts_new`
+  \\ fs[rwAllValTree_def, rwFp_pathValTree_def, option_case_eq]
+  \\ qexists_tac `Fp_uop u vNew` \\ fs[maybe_map_def]
+QED
+
+Theorem rwAllValTree_comp_right:
+  ! b v1 v2 vres insts canOpt rws.
+    rwAllValTree insts canOpt rws v2 = SOME vres ==>
+    ?insts_new.
+      rwAllValTree insts_new canOpt rws (Fp_bop b v1 v2) =
+        SOME (Fp_bop b v1 vres)
+Proof
+  Induct_on `insts` \\ rpt strip_tac
+  \\ fs[rwAllValTree_def]
+  \\ Cases_on `h` \\ fs[rwAllValTree_def, option_case_eq]
+  \\ res_tac
+  \\ first_x_assum (qspecl_then [`v1`, `b`] assume_tac)
+  \\ fs[]
+  \\ qexists_tac `(RewriteApp (Right f) n):: insts_new`
+  \\ fs[rwAllValTree_def, rwFp_pathValTree_def, maybe_map_def]
+QED
+
+Theorem rwAllValTree_comp_left:
+  ! b v1 v2 vres insts canOpt rws.
+    rwAllValTree insts canOpt rws v1 = SOME vres ==>
+    ? insts_new.
+      rwAllValTree insts_new canOpt rws (Fp_bop b v1 v2) =
+        SOME (Fp_bop b vres v2)
+Proof
+  Induct_on `insts` \\ rpt strip_tac
+  \\ fs[rwAllValTree_def]
+  \\ Cases_on `h` \\ fs[rwAllValTree_def, option_case_eq]
+  \\ res_tac
+  \\ first_x_assum (qspecl_then [`v2`, `b`] assume_tac)
+  \\ fs[]
+  \\ qexists_tac `(RewriteApp (Left f) n):: insts_new`
+  \\ fs[rwAllValTree_def, rwFp_pathValTree_def, maybe_map_def]
+QED
+
+Theorem rwAllValTree_comp_terop_l:
+  ! v vres v2 v3 insts canOpt rws t.
+    rwAllValTree insts canOpt rws v = SOME vres ==>
+    ? insts_new.
+      rwAllValTree insts_new canOpt rws (Fp_top t v v2 v3) =
+        SOME (Fp_top t vres v2 v3)
+Proof
+  Induct_on `insts` \\ rpt strip_tac \\ fs[rwAllValTree_def]
+  \\ Cases_on `h `\\ fs[rwAllValTree_def, option_case_eq]
+  \\ res_tac
+  \\ first_x_assum (qspecl_then [`v3`, `v2`, `t`] assume_tac) \\ fs[]
+  \\ qexists_tac `(RewriteApp (Left f) n)::insts_new`
+  \\ fs[rwAllValTree_def, rwFp_pathValTree_def, maybe_map_def]
+QED
+
+Theorem rwAllValTree_comp_terop_r:
+  ! v vres v1 v2 insts canOpt rws t.
+    rwAllValTree insts canOpt rws v = SOME vres ==>
+    ? insts_new.
+      rwAllValTree insts_new canOpt rws (Fp_top t v1 v2 v) =
+        SOME (Fp_top t v1 v2 vres)
+Proof
+  Induct_on `insts` \\ rpt strip_tac \\ fs[rwAllValTree_def]
+  \\ Cases_on `h `\\ fs[rwAllValTree_def, option_case_eq]
+  \\ res_tac
+  \\ first_x_assum (qspecl_then [`v2`, `v1`, `t`] assume_tac) \\ fs[]
+  \\ qexists_tac `(RewriteApp (Right f) n)::insts_new`
+  \\ fs[rwAllValTree_def, rwFp_pathValTree_def, maybe_map_def]
+QED
+
+Theorem rwAllValTree_comp_terop_c:
+  ! v vres v1 v2 insts canOpt rws t.
+    rwAllValTree insts canOpt rws v = SOME vres ==>
+    ? insts_new.
+      rwAllValTree insts_new canOpt rws (Fp_top t v1 v v2) =
+        SOME (Fp_top t v1 vres v2)
+Proof
+  Induct_on `insts` \\ rpt strip_tac \\ fs[rwAllValTree_def]
+  \\ Cases_on `h `\\ fs[rwAllValTree_def, option_case_eq]
+  \\ res_tac
+  \\ first_x_assum (qspecl_then [`v2`, `v1`, `t`] assume_tac) \\ fs[]
+  \\ qexists_tac `(RewriteApp (Center f) n)::insts_new`
+  \\ fs[rwAllValTree_def, rwFp_pathValTree_def, maybe_map_def]
+QED
+
+Theorem maybe_map_compute_thm:
+  maybe_map f v = case v of |NONE => NONE | SOME x => SOME (f x)
+Proof
+  Cases_on `v` \\ fs[maybe_map_def]
+QED
+
+Theorem rwFp_pathValTree_cond_T:
+  ! p canOpt rw v v_opt.
+    rwFp_pathValTree canOpt rw p v = SOME v_opt ==>
+    rwFp_pathValTree T rw p v = SOME v_opt
+Proof
+  reverse (Induct_on `p`) \\ fs[] \\ rpt strip_tac
+  >- (Cases_on `canOpt` \\ fs[rwFp_pathValTree_def])
+  \\ Cases_on `v`
+  \\ fs[rwFp_pathValTree_def, maybe_map_compute_thm, option_case_eq]
+  \\ res_tac \\ rveq \\ fs[]
+QED
+
+Theorem rwAllValTree_comp_scope_T:
+  ! sc v vres insts canOpt rws t.
+    rwAllValTree insts T rws v = SOME vres ==>
+    ? insts_new.
+      rwAllValTree insts_new canOpt rws (Fp_sc sc v) = SOME (Fp_sc sc vres)
+Proof
+  Induct_on `insts` \\ rpt strip_tac \\ fs[rwAllValTree_def]
+  \\ Cases_on `h `\\ fs[rwAllValTree_def, option_case_eq]
+  \\ res_tac
+  \\ first_x_assum (qspecl_then [`sc`, `vNew`, `vres`, `canOpt`, `rws`] assume_tac) \\ fs[]
+  \\ res_tac
+  \\ qexists_tac `(RewriteApp (Center f) n)::insts_new`
+  \\ Cases_on `sc`
+  \\ imp_res_tac rwFp_pathValTree_cond_T
+  \\ fs[rwAllValTree_def, rwFp_pathValTree_def, maybe_map_def]
+QED
+
+Theorem rwAllValTree_comp_scope:
+  ! sc v vres insts canOpt rws t.
+    rwAllValTree insts canOpt rws v = SOME vres ==>
+    ? insts_new.
+      rwAllValTree insts_new canOpt rws (Fp_sc sc v) = SOME (Fp_sc sc vres)
+Proof
+  Induct_on `insts` \\ rpt strip_tac \\ fs[rwAllValTree_def]
+  \\ Cases_on `h `\\ fs[rwAllValTree_def, option_case_eq]
+  \\ res_tac
+  \\ first_x_assum
+      (qspecl_then [`sc`, `vNew`, `vres`, `canOpt`, `rws`] assume_tac) \\ fs[]
+  \\ res_tac
+  \\ qexists_tac `(RewriteApp (Center f) n)::insts_new`
+  \\ Cases_on `sc`
+  \\ imp_res_tac rwFp_pathValTree_cond_T
+  \\ fs[rwAllValTree_def, rwFp_pathValTree_def, maybe_map_def]
+QED
+
+Theorem rwAllValTree_cond_T:
+  ! insts. (! canOpt rws v v_opt.
+    rwAllValTree insts canOpt rws v = SOME v_opt ==>
+    rwAllValTree insts T rws v = SOME v_opt)
+Proof
+  Induct_on `insts` \\ rpt strip_tac \\ fs[rwAllValTree_def]
+  \\ Cases_on `h` \\ fs[rwAllValTree_def, option_case_eq]
+  \\ imp_res_tac rwFp_pathValTree_cond_T
+  \\ asm_exists_tac \\ fs[]
+  \\ first_x_assum irule \\ asm_exists_tac \\ fs[]
+QED
+
+Theorem rwAllValTree_chaining_exact:
+  !v1 v2 v3 insts1 insts2 canOpt rws.
+    rwAllValTree insts1 canOpt rws v1 = SOME v2 /\
+    rwAllValTree insts2 canOpt rws v2 = SOME v3 ==>
+    rwAllValTree (APPEND insts1 insts2) canOpt rws v1 = SOME v3
+Proof
+  Induct_on `insts1` \\ rpt strip_tac
+  \\ fs[rwAllValTree_def]
+  \\ Cases_on `h` \\ fs[rwAllValTree_def, option_case_eq]
+QED
+
+Theorem rwAllValTree_chaining:
+  ! insts1 v1 v2 v3 insts2 canOpt rws.
+    rwAllValTree insts1 canOpt rws v1 = SOME v2 /\
+    rwAllValTree insts2 canOpt rws v2 = SOME v3 ==>
+    ?insts3. rwAllValTree insts3 canOpt rws v1 = SOME v3
+Proof
+  metis_tac[rwAllValTree_chaining_exact]
+QED
+
+(**
+ EXPRESSION REWRITING THEOREMS
+
+(**
+  Sanity lemma: rewriting on expressions does not introduce new variables
+**)
+local
+  val varMatch_tac =
+      imp_res_tac (ONCE_REWRITE_RULE [SUBSET_DEF] FRANGE_FUPDATE_SUBSET)
+      \\ fs[matchExpr_def, matchesCexpr_def, option_case_eq, usedVarsExp_def, flookup_thm]
+      \\ rveq
+      \\ fs[IN_UNION, usedVarsExp_def, SUBSET_DEF];
+in
+Theorem image_subst_is_usedVars
+  `(! e subst s_init pat.
+   matchesExpr pat e s_init = SOME subst ==>
+   !e_sub. e_sub IN (FRANGE subst) ==>
+   e_sub IN (FRANGE s_init) \/
+   usedVarsExp (e_sub) SUBSET (usedVarsExp e))
+  /\
+  (! c subst s_init cpat.
+       matchesCexpr cpat c s_init = SOME subst ==>
+       ! e_sub. e_sub IN (FRANGE subst) ==>
+       e_sub IN (FRANGE s_init) \/
+       usedVarsExp (e_sub) SUBSET (usedVarsCexp c))
+  /\
+  (!l. l = (l:expr list) ==> T)`
+  (ho_match_mp_tac expr_induction
+  \\ rpt strip_tac \\ fs[] \\ rpt strip_tac
+  \\ (Cases_on `pat` ORELSE Cases_on `cpat`)
+  \\ fs[matchesExpr_def, matchesCexpr_def, option_case_eq] \\ rveq
+  \\ res_tac
+  \\ varMatch_tac)
+end;
+
+Theorem usedVars_from_image_subst
+  `!pat.
+    (! e subst.
+      appExpr pat subst = SOME e ==>
+      usedVarsExp e SUBSET
+        { v | ?n e. FLOOKUP subst n = SOME e /\ v IN usedVarsExp e})
+    /\
+    (! c subst.
+      appCexpr pat subst = SOME c ==>
+      usedVarsCexp c SUBSET
+        { v | ? n e. FLOOKUP subst n = SOME e /\ v IN usedVarsExp e})`
+  (Induct_on `pat` \\ rpt strip_tac
+  \\ fs[appExpr_def, option_case_eq, usedVarsExp_def, SUBSET_DEF]
+  \\ rpt strip_tac \\ rveq \\ fs[Once usedVarsExp_def]
+  \\ asm_exists_tac \\ fs[]);
+
+Theorem rewrite_preserves_usedVars
+  `(!e e_new lhs rhs subst.
+      matchesExpr lhs e FEMPTY = SOME subst /\
+      appExpr rhs subst = SOME e_new ==>
+      usedVarsExp e_new SUBSET usedVarsExp e) /\
+    (!c c_new lhs rhs subst.
+      matchesCexpr lhs c FEMPTY = SOME subst /\
+      appCexpr rhs subst = SOME c_new ==>
+      usedVarsCexp c_new SUBSET usedVarsCexp c)`
+  (conj_tac \\ rpt strip_tac
+  \\ irule SUBSET_TRANS
+  \\ imp_res_tac usedVars_from_image_subst
+  \\ asm_exists_tac \\ fs[]
+  \\ imp_res_tac image_subst_is_usedVars
+  \\ fs[FRANGE_FEMPTY, SUBSET_DEF]
+  \\ rpt strip_tac
+  \\ fs[FRANGE_FLOOKUP]
+  \\ res_tac);
+
+Theorem matchExpr_preserving
+  `! p.
+    (! e s1 s2.
+      matchesExpr p e s1 = SOME s2 ==>
+      ! n val.
+        FLOOKUP s1 n = SOME val ==> FLOOKUP s2 n = SOME val)
+  /\
+    (! ce s1 s2.
+      matchesCexpr p ce s1 = SOME s2 ==>
+      ! n val.
+        FLOOKUP s1 n = SOME val ==> FLOOKUP s2 n = SOME val)`
+  (Induct_on `p`
+  \\ rpt strip_tac \\ fs[]
+  \\ (Cases_on `ce` ORELSE Cases_on `e`)
+  \\ fs[matchesExpr_def, matchesCexpr_def] \\ rpt strip_tac
+  \\ res_tac
+  \\ res_tac
+  \\ fs[option_case_eq] \\ rveq \\ fs[]
+  \\ irule FLOOKUP_SUBMAP \\ asm_exists_tac \\ fs[flookup_thm]);
+
+Theorem appExpr_weakening
+  `! p.
+      (! e s1 s2.
+        (! n val. FLOOKUP s1 n = SOME val ==> FLOOKUP s2 n = SOME val) /\
+        appExpr p s1 = SOME e ==>
+        appExpr p s2 = SOME e)
+  /\
+    (! ce s1 s2.
+      (! n val. FLOOKUP s1 n = SOME val ==> FLOOKUP s2 n = SOME val) /\
+      appCexpr p s1 = SOME ce ==>
+      appCexpr p s2 = SOME ce)`
+  (Induct_on `p`
+  \\ rpt strip_tac \\ fs[]
+  \\ fs[appExpr_def, pair_case_eq, option_case_eq]
+  \\ res_tac \\ fs[]);
+
+val exprSolve_tac =
+  (let
+    val thms = CONJ_LIST 2 (SIMP_RULE std_ss [FORALL_AND_THM] appExpr_weakening)
+  in
+  (irule (hd thms) ORELSE irule (hd (tl thms)))
+  end)
+  \\ once_rewrite_tac [CONJ_COMM]
+  \\ asm_exists_tac \\ fs[]
+  \\ rpt strip_tac
+  \\ imp_res_tac matchExpr_preserving \\ fs[];
+
+Theorem subst_pat_is_exp
+  `! p.
+    (! e s1 s2.
+          matchesExpr p e s1 = SOME s2 ==>
+          appExpr p s2 = SOME e)
+  /\
+    (! ce s1 s2.
+          matchesCexpr p ce s1 = SOME s2 ==>
+          appCexpr p s2 = SOME ce)`
+  (Induct_on `p`
+  \\ rpt strip_tac \\ fs[] \\ rpt strip_tac
+  \\ (Cases_on `e` ORELSE Cases_on `ce`)
+  \\ fs[matchesExpr_def, matchesCexpr_def, option_case_eq]
+  \\ rveq \\ fs[appExpr_def, FLOOKUP_UPDATE]
+  \\ res_tac \\ fs[]
+  \\ rpt conj_tac \\ exprSolve_tac);
+**)
+
+val _ = export_theory();
